SP1CleanTest/Core/HostChecks.lean
@@ -74,9 +74,9 @@ def evaluateProgram (program : Circuit Fp Unit) (inputs : List Fp)
         | _ => false
       else if interaction.channel.name == "sp1.native.hint_word" then
         match (interaction.msg.map env).toList with
-        | [a, b, c, d, e, f, w, x, y, z] =>
+        | [a, b, c, d, e, f, w, x, y, z, last] =>
           [a, b, c, d, e, f, w, x, y, z].all (fun limb => limb.val < 65536) &&
-            0 < a.val + b.val * 65536 + c.val * 65536 ^ 2
+            0 < a.val + b.val * 65536 + c.val * 65536 ^ 2 && (last == 0 || last == 1)
         | _ => false
       else ["sp1.native.hint_queue_state", "SP1State", "SP1Exit", "SP1Syscall", "SP1PublicValues", "sp1.native.host_call",
         "sp1.native.commit_state", "sp1.native.deferred_state", "sp1.native.host_ram_access"].contains
